Add raw indexing
I'm calling "raw indexing" the act of grabbing the correct
number of bytes for the dtype out of an array at a given index
and returning the decoded element of the type. This will
form the basis for real NumPy indexing.

TensorLib/NumpyRepr.lean
@@ -1,7 +1,6 @@
-import Init.System.IO
 import Init.System.FilePath
+import Init.System.IO
 import Mathlib.Tactic
-import TensorLib.TensorElement
 
 /-!
 We largely duplicate the NumPy representation of tensors.
@@ -14,8 +13,198 @@ In addition to being efficient, this allows us to directly parse .npy input file
 
 namespace TensorLib
 
+abbrev Err := Except String
+
+instance [BEq a] : BEq (Err a) where
+  beq x y := match x, y with
+  | .ok x, .ok y => x == y
+  | .error x, .error y => x == y
+  | _, _ => false
+
+section Util
+
+-- We generally have huge tensors, so don't show them by default
+instance : Repr ByteArray where
+  reprPrec x _ :=
+    let s := toString x.size
+    s!"ByteArray of size {s}"
+
+-- UInt8, UInt64, etc don't work well with bv_decide yet. It's coming
+abbrev BV8 := BitVec 8
+abbrev BV16 := BitVec 16
+abbrev BV32 := BitVec 32
+abbrev BV64 := BitVec 64
+
+def BV16ToBytes (n : BV16) : BV8 × BV8 :=
+  let n0 := (n >>> 0o00 &&& 0xFF).truncate 8
+  let n1 := (n >>> 0o10 &&& 0xFF).truncate 8
+  (n0, n1)
+
+def BytesToBV16 (x0 x1 : BV8) : BV16 :=
+  (x0.zeroExtend 16 <<< 0o00) |||
+  (x1.zeroExtend 16 <<< 0o10)
+
+def BV32ToBytes (n : BV32) : BV8 × BV8 × BV8 × BV8 :=
+  let n0 := (n >>> 0o00 &&& 0xFF).truncate 8
+  let n1 := (n >>> 0o10 &&& 0xFF).truncate 8
+  let n2 := (n >>> 0o20 &&& 0xFF).truncate 8
+  let n3 := (n >>> 0o30 &&& 0xFF).truncate 8
+  (n0, n1, n2, n3)
+
+def BytesToBV32 (x0 x1 x2 x3 : BV8) : BV32 :=
+  (x0.zeroExtend 32 <<< 0o00) |||
+  (x1.zeroExtend 32 <<< 0o10) |||
+  (x2.zeroExtend 32 <<< 0o20) |||
+  (x3.zeroExtend 32 <<< 0o30)
+
+def BV64ToBytes (n : BV64) : BV8 × BV8 × BV8 × BV8 × BV8 × BV8 × BV8 × BV8 :=
+  let n0 := (n >>> 0o00 &&& 0xFF).truncate 8
+  let n1 := (n >>> 0o10 &&& 0xFF).truncate 8
+  let n2 := (n >>> 0o20 &&& 0xFF).truncate 8
+  let n3 := (n >>> 0o30 &&& 0xFF).truncate 8
+  let n4 := (n >>> 0o40 &&& 0xFF).truncate 8
+  let n5 := (n >>> 0o50 &&& 0xFF).truncate 8
+  let n6 := (n >>> 0o60 &&& 0xFF).truncate 8
+  let n7 := (n >>> 0o70 &&& 0xFF).truncate 8
+  (n0, n1, n2, n3, n4, n5, n6, n7)
+
+def BytesToBV64 (x0 x1 x2 x3 x4 x5 x6 x7 : BV8) : BV64 :=
+  (x0.zeroExtend 64 <<< 0o00) |||
+  (x1.zeroExtend 64 <<< 0o10) |||
+  (x2.zeroExtend 64 <<< 0o20) |||
+  (x3.zeroExtend 64 <<< 0o30) |||
+  (x4.zeroExtend 64 <<< 0o40) |||
+  (x5.zeroExtend 64 <<< 0o50) |||
+  (x6.zeroExtend 64 <<< 0o60) |||
+  (x7.zeroExtend 64 <<< 0o70)
+
+theorem BV64BytesRoundTrip (n : BV64) :
+  let (x0, x1, x2, x3, x4, x5, x6, x7) := BV64ToBytes n
+  let n' := BytesToBV64 x0 x1 x2 x3 x4 x5 x6 x7
+  n = n' := by
+    unfold BV64ToBytes BytesToBV64
+    bv_decide
+
+theorem BV64BytesRoundTrip1 (x0 x1 x2 x3 x4 x5 x6 x7 : BV8) :
+  let n := BytesToBV64 x0 x1 x2 x3 x4 x5 x6 x7
+  let (x0', x1', x2', x3', x4', x5', x6', x7') := BV64ToBytes n
+  x0 = x0' &&
+  x1 = x1' &&
+  x2 = x2' &&
+  x3 = x3' &&
+  x4 = x4' &&
+  x5 = x5' &&
+  x6 = x6' &&
+  x7 = x7' := by
+    unfold BV64ToBytes BytesToBV64
+    bv_decide
+
+end Util
+
+namespace NumpyDtype
+
+inductive ByteOrder where
+| native
+| littleEndian
+| bigEndian
+| notApplicable
+deriving BEq, Repr
+
+namespace ByteOrder
+
+def toChar (x : ByteOrder) := match x with
+| native => '='
+| littleEndian => '<'
+| bigEndian => '>'
+| notApplicable => '|'
+
+def fromChar (c : Char) : Err ByteOrder := match c with
+| '=' => .ok native
+| '<' => .ok littleEndian
+| '>' => .ok bigEndian
+| '|' => .ok notApplicable
+| _ => .error s!"can't parse byte order: {c}"
+
+def UInt8ToBV8 (n : UInt8) : BV8 := BitVec.ofFin n.val
+def BV8ToUInt8 (n : BV8) : UInt8 := UInt8.ofNat n.toFin
+
+private def getBV16Aux (order : ByteOrder) (x0 x1 : BV8) : Err BV16 :=
+  match order with
+  | .notApplicable | .native => .error "illegal byte order"
+  | .littleEndian => .ok (BytesToBV16 x0 x1)
+  | .bigEndian => .ok (BytesToBV16 x1 x0)
+
+def getBV16 (order : ByteOrder) (x : ByteArray) (startIndex : Nat) : Err BV16 :=
+  let n := startIndex
+  if H7 : n + 1 < x.size then
+    let H0 : n + 0 < x.size := by linarith
+    let H1 : n + 1 < x.size := by linarith
+    let x0 := UInt8ToBV8 $ x.get (Fin.mk _ H0)
+    let x1 := UInt8ToBV8 $ x.get (Fin.mk _ H1)
+    getBV16Aux order x0 x1
+  else .error "Index out of range"
+
+private def getBV32Aux (order : ByteOrder) (x0 x1 x2 x3 : BV8) : Err BV32 :=
+  match order with
+  | .notApplicable | .native => .error "illegal byte order"
+  | .littleEndian => .ok (BytesToBV32 x0 x1 x2 x3)
+  | .bigEndian => .ok (BytesToBV32 x3 x2 x1 x0)
+
+def getBV32 (order : ByteOrder) (x : ByteArray) (startIndex : Nat) : Err BV32 :=
+  let n := startIndex
+  if H7 : n + 3 < x.size then
+    let H0 : n + 0 < x.size := by linarith
+    let H1 : n + 1 < x.size := by linarith
+    let H2 : n + 2 < x.size := by linarith
+    let H3 : n + 3 < x.size := by linarith
+    let x0 := UInt8ToBV8 $ x.get (Fin.mk _ H0)
+    let x1 := UInt8ToBV8 $ x.get (Fin.mk _ H1)
+    let x2 := UInt8ToBV8 $ x.get (Fin.mk _ H2)
+    let x3 := UInt8ToBV8 $ x.get (Fin.mk _ H3)
+    getBV32Aux order x0 x1 x2 x3
+  else .error "Index out of range"
+
+private def getBV64Aux (order : ByteOrder) (x0 x1 x2 x3 x4 x5 x6 x7 : BV8) : Err BV64 :=
+  match order with
+  | .notApplicable | .native => .error "illegal byte order"
+  | .littleEndian => .ok (BytesToBV64 x0 x1 x2 x3 x4 x5 x6 x7)
+  | .bigEndian => .ok (BytesToBV64 x7 x6 x5 x4 x3 x2 x1 x0)
+
+def getBV64 (order : ByteOrder) (x : ByteArray) (startIndex : Nat) : Err BV64 :=
+  let n := startIndex
+  if H7 : n + 7 < x.size then
+    let H0 : n + 0 < x.size := by linarith
+    let H1 : n + 1 < x.size := by linarith
+    let H2 : n + 2 < x.size := by linarith
+    let H3 : n + 3 < x.size := by linarith
+    let H4 : n + 4 < x.size := by linarith
+    let H5 : n + 5 < x.size := by linarith
+    let H6 : n + 6 < x.size := by linarith
+    let x0 := UInt8ToBV8 $ x.get (Fin.mk _ H0)
+    let x1 := UInt8ToBV8 $ x.get (Fin.mk _ H1)
+    let x2 := UInt8ToBV8 $ x.get (Fin.mk _ H2)
+    let x3 := UInt8ToBV8 $ x.get (Fin.mk _ H3)
+    let x4 := UInt8ToBV8 $ x.get (Fin.mk _ H4)
+    let x5 := UInt8ToBV8 $ x.get (Fin.mk _ H5)
+    let x6 := UInt8ToBV8 $ x.get (Fin.mk _ H6)
+    let x7 := UInt8ToBV8 $ x.get (Fin.mk _ H7)
+    getBV64Aux order x0 x1 x2 x3 x4 x5 x6 x7
+  else .error "Index out of range"
+
+-- #guard doesn't work here. Not sure why.
+#eval
+  let n : BV64 := 0x3FFAB851EB851EB8
+  let (x0, x1, x2, x3, x4, x5, x6, x7) := BV64ToBytes n
+  -- Big-endian array layout
+  let data := ByteArray.mk (Array.mkArray8 (BV8ToUInt8 x0) (BV8ToUInt8 x1) (BV8ToUInt8 x2) (BV8ToUInt8 x3) (BV8ToUInt8 x4) (BV8ToUInt8 x5) (BV8ToUInt8 x6) (BV8ToUInt8 x7))
+  do
+    let n' <- getBV64 ByteOrder.littleEndian data 0
+    return n == n'
+
+end ByteOrder
+
 /-! The subset of types NumPy supports that we care about -/
-inductive NumpyDtype where
+inductive Name where
 | bool
 | int8
 | int16
@@ -28,12 +217,15 @@ inductive NumpyDtype where
 | float16
 | float32
 | float64
-  deriving Repr
+deriving BEq, Repr
 
-namespace NumpyDtype
+namespace Name
+
+instance : ToString Name where
+  toString x := (repr x).pretty
 
 --! Number of bytes used by each element of the given dtype
-def bytes (x: NumpyDtype): Nat := match x with
+def numBytes (x: Name): Nat := match x with
 | float64 | int64 | uint64 => 8
 | float32 | int32 | uint32 => 4
 | float16 | int16 | uint16 => 2
@@ -48,22 +240,22 @@ byte order: https://numpy.org/doc/2.1/reference/generated/numpy.dtype.byteorder.
 '<' is little endian, '|' is "not applicable" Not sure why bool showed up
 as both.
 -/
-def fromString (s : String) : Except String NumpyDtype := match s with
-| "<b1" | "|b1"=> .ok bool
-| "|i1" => .ok int8
-| "<i2" => .ok int16
-| "<i4" => .ok int32
-| "<i8" => .ok int64
-| "|u1" => .ok uint8
-| "<u2" => .ok uint16
-| "<u4" => .ok uint32
-| "<u8" => .ok uint64
-| "<f2" => .ok float16
-| "<f4" => .ok float32
-| "<f8" => .ok float64
+def fromString (s : String) : Err Name := match s with
+| "b1" => .ok bool
+| "i1" => .ok int8
+| "i2" => .ok int16
+| "i4" => .ok int32
+| "i8" => .ok int64
+| "u1" => .ok uint8
+| "u2" => .ok uint16
+| "u4" => .ok uint32
+| "u8" => .ok uint64
+| "f2" => .ok float16
+| "f4" => .ok float32
+| "f8" => .ok float64
 | _ => .error s!"Can't parse {s} as a dtype"
 
-def toString (t : NumpyDtype) : String := match t with
+def toString (t : Name) : String := match t with
 | bool => "b1"
 | int8 => "i1"
 | int16 => "i2"
@@ -77,13 +269,36 @@ def toString (t : NumpyDtype) : String := match t with
 | float32 => "f4"
 | float64 => "f8"
 
-end NumpyDtype
+end Name
 
---! Numpy disk format uses python convention for bools; True/False
-def NumpyBool.fromString (s: String): Except String Bool := match s with
-| "True" => .ok true
-| "False" => .ok false
-| _ => .error s!"Can't parse {s} as Bool"
+end NumpyDtype -- temporarily close the namespace so we don't duplicate the structure name
+
+structure NumpyDtype where
+  name : NumpyDtype.Name
+  order : NumpyDtype.ByteOrder
+deriving BEq, Repr
+
+namespace NumpyDtype
+
+def numBytes (t : NumpyDtype) := t.name.numBytes
+
+def fromString (s : String) : Err NumpyDtype :=
+  if s.length == 0 then .error "Empty dtype string" else
+  do
+    let order <- ByteOrder.fromChar (s.get 0)
+    let name <- Name.fromString (s.drop 1)
+    return { name, order }
+
+def toString (t : NumpyDtype) : String := t.order.toChar.toString.append t.name.toString
+
+-- Examples
+private def littleEndian (name : Name) : NumpyDtype := { name, order := ByteOrder.littleEndian }
+private def uint8 : NumpyDtype := { name := Name.uint8 , order := ByteOrder.notApplicable }
+private def uint16 : NumpyDtype := littleEndian Name.uint16
+private def uint32 : NumpyDtype := littleEndian Name.uint32
+private def uint64 : NumpyDtype := littleEndian Name.uint64
+
+end NumpyDtype
 
 /-!
 Shapes and strides in tensors are represented as lists, where the length of the
@@ -139,6 +354,7 @@ Strides also are empty for scalar arrays.
 -/
 abbrev Shape := List Nat
 abbrev Strides := List Nat
+abbrev Index := List Nat
 
 namespace Shape
 
@@ -160,7 +376,7 @@ so this is just the default case.
 def defaultStrides (dtype : NumpyDtype) (s : Shape) : Strides :=
   if H : s.isEmpty then [] else
   let s' := s.reverse
-  let bytes := dtype.bytes
+  let bytes := dtype.numBytes
   let rec loop (xs : List ℕ) (lastShape lastDimSize : ℕ): List ℕ := match xs with
   | [] => []
   | d :: ds =>
@@ -171,7 +387,7 @@ def defaultStrides (dtype : NumpyDtype) (s : Shape) : Strides :=
     simp [H1]
     simp at H
     exact H
-  let res : Strides := dtype.bytes :: loop s'.tail bytes (s'.head ok)
+  let res : Strides := dtype.numBytes :: loop s'.tail bytes (s'.head ok)
   res.reverse
 
 #guard defaultStrides NumpyDtype.uint32 [2] == [4]
@@ -206,15 +422,10 @@ namespace NumpyHeader
 A npy binary file has a header, some padding, then the data. This method computes the
 size of the data portion of the file.
 -/
-def dataSize (header : NumpyHeader): Nat := header.descr.bytes * header.shape.count
+def dataSize (header : NumpyHeader): Nat := header.descr.numBytes * header.shape.count
 
 end NumpyHeader
 
--- We generally have huge tensors, so don't show them by default
-instance ByteArrayRepr : Repr ByteArray where
-  reprPrec x _ :=
-    let s := toString x.size
-    s!"ByteArray of size {s}"
 
 /-!
 A NumpyRepr is the data of the tensor, along with all metadata required to do
@@ -227,7 +438,7 @@ structure NumpyRepr where
   startIndex : Nat -- Pointer to the first byte of ndarray data, called `offset` in numpy
   endIndex : Nat   -- Pointer to the byte after the last byte of ndarray data
   -- invariant: startIndex <= endIndex
-  -- invariant: endIndex - startIndex = descr.bytes * shape.count
+  -- invariant: endIndex - startIndex = header.descr.numBytes * shape.count
   -- invariant: header.endIndex <= |data|
   -- invariant: header.dataSize <= |data|
   strides : Strides
@@ -245,27 +456,92 @@ def ndim (x : NumpyRepr) : ℕ := x.shape.length
 def size (x : NumpyRepr) : ℕ := x.shape.count
 
 --! number of bytes representing each element
-def itemsize (x : NumpyRepr) : ℕ := x.header.descr.bytes
+def itemsize (x : NumpyRepr) : ℕ := x.header.descr.numBytes
 
 --! number of bytes representing the entire tensor
 def nbytes (x : NumpyRepr) : ℕ := x.itemsize * x.size
-
-section Shape
-
-abbrev M a := Except String a
 
 /-!
 Reshaping a tensor is just re-interpreting the elements in
 a different order. This will also impact the iteration order/strides
 when we implement those.
 -/
-def reshape (x : NumpyRepr) (shape : Shape) : M NumpyRepr := do
+def reshape (x : NumpyRepr) (shape : Shape) : Err NumpyRepr := do
   if x.shape.count == shape.count then
     return { x with header.shape := shape }
   else
     .error "Reshaping must have the same number of implied elements"
 
-end Shape
+class TensorElement (a: Type) where
+  numBytes : Nat
+  fromByteArray (byteOrder : NumpyDtype.ByteOrder) (arr : ByteArray) (startIndex : Nat) : Err a
+
+namespace TensorElement
+
+-- Style of repeating the arguments to a class followed by variables was
+-- suggested by Lean office hours folks
+-- variable (a: Type)
+-- variable [Add a][Sub a][Mul a][Neg a]
+
+-- ...Lots of definitions here using the variables above...
+
+instance BV16 : TensorElement BV16 where
+  numBytes := 2
+  fromByteArray byteOrder arr startIndex :=
+    if arr.size < startIndex + 2 -- would like to use `numBytes` but it's not resolving
+    then .error "Wrong size array"
+    else byteOrder.getBV16 arr startIndex
+
+instance BV32: TensorElement BV32 where
+  numBytes := 4
+  fromByteArray byteOrder arr startIndex :=
+    if arr.size < startIndex + 4
+    then .error "Wrong size array"
+    else byteOrder.getBV32 arr startIndex
+
+instance BV64: TensorElement BV64 where
+  numBytes := 8
+  fromByteArray byteOrder arr startIndex :=
+    if arr.size < startIndex + 8
+    then .error "Wrong size array"
+    else byteOrder.getBV64 arr startIndex
+
+end TensorElement
+
+
+namespace Index
+
+-- Indexing utility
+private def start (strides : Strides) (index : Index) : Err ℕ :=
+  match strides, index with
+  | [], [] => .error "Can not index with empty list"
+  | [], _ :: _ | _ :: _, [] => .error "Unequal lengths: strides and index"
+  | stride :: strides, i :: index => (start strides index).map (. + i * stride)
+
+-- Get a single value from the tensor.
+-- TODO: Replace get! with the Fin version. I tried this for a couple hours
+-- and failed.
+private def getBytes! (x : NumpyRepr) (index : Index) : Err (List UInt8) := do
+  let gap <- start x.strides index
+  let i := x.startIndex + gap
+  let rec loop (n : ℕ) (acc : List UInt8) : List UInt8 :=
+    match n with
+    | 0 => acc
+    | n + 1 => loop n (x.data.get! (i + n) :: acc)
+  return loop x.itemsize []
+
+-- This is a blind index into the array, disregarding the shape.
+def rawIndex (typ : TensorElement a) (x : NumpyRepr) (index : Nat) : Err a :=
+  if typ.numBytes != x.itemsize then .error "byte size mismatch" else -- TODO: Lift this check out so we only do it once
+  typ.fromByteArray x.header.descr.order x.data (x.startIndex + (index * typ.numBytes))
+
+end Index
+
+def transpose (x : NumpyRepr) : NumpyRepr :=
+  let shape := x.header.shape.reverse
+  let header := { x.header with shape }
+  let strides := x.strides.reverse
+  { x with header, strides }
 
 /-!
 Broadcasting is a convenience and performance trick to allow operations that expect the same
@@ -374,13 +650,13 @@ structure ParsingState where
 
 abbrev PState (T : Type) := EStateM String ParsingState T
 
-instance : MonadLiftT (Except String) PState where
+instance : MonadLiftT Err PState where
   monadLift x := match x with
   | .ok x => .ok x
   | .error x => .error x
 
 -- Except is nicer sometimes
-def resultExcept {σ : Type} (x : EStateM.Result String σ a) : Except String a := match x with
+def resultExcept {σ : Type} (x : EStateM.Result String σ a) : Err a := match x with
 | .ok x _ => .ok x
 | .error x _ => .error x
 
@@ -388,6 +664,12 @@ variable {T : Type}
 
 def debug (msg : String) : PState Unit := do
   modify (fun s => { s with debug := msg :: s.debug })
+
+-- Numpy disk format uses python convention for bools; True/False
+private def numpyBool (s: String): Err Bool := match s with
+| "True" => .ok true
+| "False" => .ok false
+| _ => .error s!"Can't parse {s} as Bool"
 
 -- Whitespace is under-specified in the docs linked above, but I think
 -- Lean's isWhitespace will be fine here. I have never seen a non 0x20
@@ -471,7 +753,7 @@ def parseHeader : PState (UInt8 × UInt8) := do
   let s <- get
   let b := s.source
   if s.index != 0 then .error "Illegal start index"
-  if b.size < 10 then .error "Buffer too small"
+  if b.size < 10 then .error s!"Buffer too small: {b.size}"
   if b[0]! != 0x93 then .error s!"Invalid first byte: {b[0]!}"
   if b[1]! != 'N'.toUInt8 then .error "Invalid second byte"
   if b[2]! != 'U'.toUInt8 then .error "Invalid third byte"
@@ -496,7 +778,7 @@ def parseOneMetadata : PState Unit := do
     modify (fun s => { s with descr := some d })
   else if id == "fortran_order" then
     let v <- parseToken
-    let b <- liftM (NumpyBool.fromString v)
+    let b <- liftM (numpyBool v)
     modify (fun s => { s with fortranOrder := b })
   else if id == "shape" then
     let shape <- parseShape
@@ -527,11 +809,11 @@ def parseNumpyRepr : PState NumpyRepr := do
     return repr
   | _, _, _ => .error "Can't parse a metadata value"
 
-def parse (buffer : ByteArray) : Except String NumpyRepr := do
+def parse (buffer : ByteArray) : Err NumpyRepr := do
   let init := ParsingState.mk buffer 0 0 none none none []
   resultExcept $ parseNumpyRepr.run init
 
-def parseFile (path: System.FilePath) : IO (Except String NumpyRepr) := do
+def parseFile (path: System.FilePath) : IO (Err NumpyRepr) := do
   let buffer <- IO.FS.readBinFile path
   return parse buffer
 
@@ -591,6 +873,53 @@ end Save
 
 def save! (repr : NumpyRepr) (file : System.FilePath) : IO Unit :=
   IO.FS.writeBinFile file repr.toByteArray!
+
+section Test
+
+def DEBUG := false
+def debugPrint {a : Type} [Repr a] (s : a) : IO Unit := if DEBUG then IO.print (Std.Format.pretty (repr s)) else return ()
+def debugPrintln {a : Type} [Repr a] (s : a) : IO Unit := do
+  debugPrint s
+  if DEBUG then IO.print "\n" else return ()
+
+-- Caller must remove the temp file
+def saveNumpyArray (expr : String) : IO System.FilePath := do
+  let (_root_, file) <- IO.FS.createTempFile
+  let expr := s!"import numpy as np; x = {expr}; np.save('{file}', x)"
+  let output <- IO.Process.output { cmd := "/usr/bin/env", args := ["python3", "-c", expr].toArray }
+  let _ <- debugPrintln output.stdout
+  let _ <- debugPrintln output.stderr
+  -- `np.save` appends `.npy` to the file
+  return file.addExtension "npy"
+
+def testTensorElementBV {n : Nat} (w : TensorElement (BitVec n)) (dtype : String) : IO Bool := do
+  let file <- saveNumpyArray s!"np.arange(20, dtype='{dtype}').reshape(5, 4)"
+  let arr <- Parse.parseFile file
+  let _ <- debugPrintln file
+  let _ <- debugPrintln arr
+  let _ <- IO.FS.removeFile file
+  let expected : List (BitVec n) := List.range 20
+  let actual := arr.bind (fun arr => do
+    let rev <- Nat.foldM (fun i acc => (Index.rawIndex w arr i).map (fun i => i :: acc)) [] 20
+    return rev.reverse
+  )
+  let _ <- debugPrintln actual
+  match actual with
+  | .error _ => return false
+  | .ok actual => return expected == actual
+
+-- Asserting true/false here would be great
+#eval testTensorElementBV TensorElement.BV16 "uint16" -- expect true
+#eval testTensorElementBV TensorElement.BV32 "uint16" -- expect false
+#eval testTensorElementBV TensorElement.BV64 "uint16" -- expect false
+#eval testTensorElementBV TensorElement.BV16 "uint32" -- expect false
+#eval testTensorElementBV TensorElement.BV32 "uint32" -- expect true
+#eval testTensorElementBV TensorElement.BV64 "uint32" -- expect false
+#eval testTensorElementBV TensorElement.BV16 "uint64" -- expect false
+#eval testTensorElementBV TensorElement.BV32 "uint64" -- expect false
+#eval testTensorElementBV TensorElement.BV64 "uint64" -- expect true
+
+end Test
 
 end NumpyRepr
 end TensorLib
